prove add_loop spec refinement

examples/loops_proofs.v
@@ -33,14 +33,44 @@ Definition add_loop_letRec_lrt
                (fun _ : {_ : bitvector 64 & unit} =>
                 LRT_Ret {_ : bitvector 64 & unit})))).
 
-Definition add_loop_noErrors_letRec : lrtToType add_loop_lrt := fun _ _ =>
-   letRecM (lrts:=LRT_Cons add_loop_letRec_lrt LRT_Nil)
-           (fun _ => (fun _ _ _ _ => noErrorsSpec, tt))
-           (fun _ => noErrorsSpec).
 
 Lemma no_errors_add_loop : refinesFun add_loop (fun _ _ => noErrorsSpec).
 Proof.
-  transitivity add_loop_noErrors_letRec; try reflexivity.
-  unfold add_loop, add_loop__tuple_fun, add_loop_noErrors_letRec, noErrorsSpec.
+  transitivity ((fun _ _ => letRecM (lrts:=LRT_Cons add_loop_letRec_lrt LRT_Nil)
+                                    (fun _ => (fun _ _ _ _ => noErrorsSpec, tt))
+                                    (fun _ => noErrorsSpec)) : lrtToType add_loop_lrt);
+               try reflexivity.
+  unfold add_loop, add_loop__tuple_fun, noErrorsSpec.
   prove_refinement.
+Qed.
+
+
+Definition add_loop_spec : lrtToType add_loop_lrt
+  := fun x y => returnM (existT _ (bvAdd 64 (projT1 x) (projT1 y)) tt).
+
+Lemma add_loop_spec_ref : refinesFun add_loop add_loop_spec.
+Proof.
+  transitivity (fun x y => letRecM (lrts:=LRT_Cons add_loop_letRec_lrt LRT_Nil)
+                                   (fun _ => (fun _ _ ret i => add_loop_spec ret i, tt))
+                                   (fun _ => add_loop_spec x y));
+               try reflexivity.
+  unfold add_loop, add_loop__tuple_fun, add_loop_spec, noErrorsSpec.
+  prove_refinement; cbn [ projT1 ].
+  - f_equal.
+    rewrite bvAdd_assoc.
+    rewrite (bvAdd_comm _ (projT1 a4)).
+    rewrite <- (bvAdd_assoc _ _ _ (projT1 a4)).
+    unfold true, false.
+    (* The next three lines could just be replaced by `vm_compute bvAdd at 3`,
+       but then `Qed` hangs... *)
+    assert (bvAdd 64 (bvLit 64 1) (bvLit 64 (-1)) = bvLit 64 0) as H by reflexivity.
+    vm_compute bvLit in H.
+    rewrite H.
+    rewrite bvAdd_id_l.
+    reflexivity.
+  - rewrite bvEq_wrapped_bool, isBvule_def_opp in e_if.
+    rewrite isBvule_n_zero in e_if.
+    rewrite e_if, bvAdd_id_r.
+    destruct a3 as [ projT1_a3 u ]; destruct u; simpl.
+    reflexivity.
 Qed.
